example_userbase.thy
@@ -1,5 +1,5 @@
 theory example_userbase
-imports invariant_simps
+  imports invariant_simps
 begin
 
 
@@ -8,7 +8,7 @@ begin
 (* ^^^^ *)
 
 datatype val =
-    String string
+  String string
   | UserId int
   | Bool bool
   | Undef
@@ -18,7 +18,7 @@ datatype val =
 fun stringval where
   "stringval (String s) = s"
 | "stringval _ = ''''"
-  
+
 record localState = 
   ls_pc :: nat
   ls_u :: val
@@ -27,14 +27,14 @@ record localState =
   ls_exists :: bool
 
 definition lsInit :: "localState" where
-"lsInit = \<lparr>
+  "lsInit = \<lparr>
   ls_pc = 0,
   ls_u = Undef,
   ls_name = '''',
   ls_mail = '''',
   ls_exists = False
 \<rparr>"
-  
+
 (*
   querySpec :: "operation \<Rightarrow> 'any list \<Rightarrow> 'any operationContext \<Rightarrow> 'any \<Rightarrow> bool"
   procedure :: "procedureName \<Rightarrow> 'any list \<rightharpoonup> ('localState \<times> ('localState, 'any) procedureImpl)"
@@ -84,58 +84,58 @@ thm conjI
 thm name_distinct2[intro]
 
 lemma names_distinct3[simp]:
-"users_name_assign \<noteq> users_mail_assign"
-"users_name_assign \<noteq> users_contains_key"
-"users_name_assign \<noteq> users_remove"
-"users_name_assign \<noteq> users_name_get"
-"users_name_assign \<noteq> users_mail_get"
-"users_name_assign \<noteq> registerUser "
-"users_name_assign \<noteq> updateMail "
-"users_name_assign \<noteq> removeUser "
-"users_name_assign \<noteq> getUser"
-"users_mail_assign \<noteq> users_contains_key"
-"users_mail_assign \<noteq> users_remove"
-"users_mail_assign \<noteq> users_name_get"
-"users_mail_assign \<noteq> users_mail_get"
-"users_mail_assign \<noteq> registerUser "
-"users_mail_assign \<noteq> updateMail "
-"users_mail_assign \<noteq> removeUser "
-"users_mail_assign \<noteq> getUser "
-"users_contains_key \<noteq> users_remove"
-"users_contains_key \<noteq> users_name_get"
-"users_contains_key \<noteq> users_mail_get"
-"users_contains_key \<noteq> registerUser"
-"users_contains_key \<noteq> updateMail"
-"users_contains_key \<noteq> removeUser"
-"users_contains_key \<noteq> getUser"
-"users_remove \<noteq> users_name_get"
-"users_remove \<noteq> users_mail_get"
-"users_remove \<noteq> registerUser"
-"users_remove \<noteq> updateMail"
-"users_remove \<noteq> removeUser"
-"users_remove \<noteq> getUser"
-"users_name_get \<noteq> users_mail_get"
-"users_name_get \<noteq> registerUser "
-"users_name_get \<noteq> updateMail "
-"users_name_get \<noteq> removeUser "
-"users_name_get \<noteq> getUser "
-"users_mail_get \<noteq> registerUser"
-"users_mail_get \<noteq> updateMail "
-"users_mail_get \<noteq> removeUser "
-"users_mail_get \<noteq> getUser "
-"registerUser \<noteq> updateMail"
-"registerUser \<noteq> removeUser "
-"registerUser \<noteq> getUser "
-"updateMail \<noteq> removeUser "
-"updateMail \<noteq> getUser "
-"removeUser \<noteq> getUser"
+  "users_name_assign \<noteq> users_mail_assign"
+  "users_name_assign \<noteq> users_contains_key"
+  "users_name_assign \<noteq> users_remove"
+  "users_name_assign \<noteq> users_name_get"
+  "users_name_assign \<noteq> users_mail_get"
+  "users_name_assign \<noteq> registerUser "
+  "users_name_assign \<noteq> updateMail "
+  "users_name_assign \<noteq> removeUser "
+  "users_name_assign \<noteq> getUser"
+  "users_mail_assign \<noteq> users_contains_key"
+  "users_mail_assign \<noteq> users_remove"
+  "users_mail_assign \<noteq> users_name_get"
+  "users_mail_assign \<noteq> users_mail_get"
+  "users_mail_assign \<noteq> registerUser "
+  "users_mail_assign \<noteq> updateMail "
+  "users_mail_assign \<noteq> removeUser "
+  "users_mail_assign \<noteq> getUser "
+  "users_contains_key \<noteq> users_remove"
+  "users_contains_key \<noteq> users_name_get"
+  "users_contains_key \<noteq> users_mail_get"
+  "users_contains_key \<noteq> registerUser"
+  "users_contains_key \<noteq> updateMail"
+  "users_contains_key \<noteq> removeUser"
+  "users_contains_key \<noteq> getUser"
+  "users_remove \<noteq> users_name_get"
+  "users_remove \<noteq> users_mail_get"
+  "users_remove \<noteq> registerUser"
+  "users_remove \<noteq> updateMail"
+  "users_remove \<noteq> removeUser"
+  "users_remove \<noteq> getUser"
+  "users_name_get \<noteq> users_mail_get"
+  "users_name_get \<noteq> registerUser "
+  "users_name_get \<noteq> updateMail "
+  "users_name_get \<noteq> removeUser "
+  "users_name_get \<noteq> getUser "
+  "users_mail_get \<noteq> registerUser"
+  "users_mail_get \<noteq> updateMail "
+  "users_mail_get \<noteq> removeUser "
+  "users_mail_get \<noteq> getUser "
+  "registerUser \<noteq> updateMail"
+  "registerUser \<noteq> removeUser "
+  "registerUser \<noteq> getUser "
+  "updateMail \<noteq> removeUser "
+  "updateMail \<noteq> getUser "
+  "removeUser \<noteq> getUser"
   using name_distinct2 by auto
 
 lemmas names_distinct4[simp] = names_distinct3[symmetric]
 
 
 definition registerUserImpl :: "(localState, val) procedureImpl" where
-"registerUserImpl ls \<equiv> [
+  "registerUserImpl ls \<equiv> [
    (* 0 *) NewId (\<lambda>x. (ls\<lparr>ls_u := x, ls_pc := 1\<rparr> :: localState)),
    (* 1 *) BeginAtomic (ls\<lparr>ls_pc := 2\<rparr>),
    (* 2 *) DbOperation users_name_assign [ls_u ls, String (ls_name ls)] (\<lambda>r. ls\<lparr>ls_pc := 3\<rparr>),
@@ -145,7 +145,7 @@ definition registerUserImpl :: "(localState, val) procedureImpl" where
    ] ! ls_pc ls"
 
 definition updateMailImpl :: "(localState, val) procedureImpl" where
-"updateMailImpl ls \<equiv> [
+  "updateMailImpl ls \<equiv> [
    (* 0 *) BeginAtomic (ls\<lparr>ls_pc := 1\<rparr>),
    (* 1 *) DbOperation users_contains_key [ls_u ls] (\<lambda>r. ls\<lparr>ls_exists := (r = Bool True), ls_pc := 2 \<rparr>),
    (* 2 *) LocalStep (if ls_exists ls then ls\<lparr>ls_pc := 3\<rparr> else ls\<lparr>ls_pc := 4\<rparr> ),
@@ -153,17 +153,17 @@ definition updateMailImpl :: "(localState, val) procedureImpl" where
    (* 5 *) EndAtomic  (ls\<lparr>ls_pc := 6\<rparr>),
    (* 6 *) Return Undef
    ] ! ls_pc ls"   
-   
+
 definition removeUserImpl :: "(localState, val) procedureImpl" where
-"removeUserImpl ls \<equiv> [
+  "removeUserImpl ls \<equiv> [
    (* 0 *) BeginAtomic (ls\<lparr>ls_pc := 1\<rparr>),
    (* 1 *) DbOperation users_remove [ls_u ls] (\<lambda>r. ls\<lparr>ls_pc := 2 \<rparr>),
    (* 2 *) EndAtomic  (ls\<lparr>ls_pc := 3\<rparr>),
    (* 3 *) Return Undef
    ] ! ls_pc ls"
-   
+
 definition getUserImpl :: "(localState, val) procedureImpl" where
-"getUserImpl ls \<equiv> [
+  "getUserImpl ls \<equiv> [
    (* 0 *) BeginAtomic (ls\<lparr>ls_pc := 1\<rparr>),
    (* 1 *) DbOperation users_contains_key [ls_u ls] (\<lambda>r. ls\<lparr>ls_exists := (r = Bool True), ls_pc := 2 \<rparr>),
    (* 2 *) LocalStep (if ls_exists ls then ls\<lparr>ls_pc := 3\<rparr> else ls\<lparr>ls_pc := 5\<rparr> ),
@@ -172,10 +172,10 @@ definition getUserImpl :: "(localState, val) procedureImpl" where
    (* 5 *) EndAtomic  (ls\<lparr>ls_pc := 6\<rparr>),
    (* 6 *) Return (if ls_exists ls then Found (ls_name ls) (ls_mail ls) else NotFound )
    ] ! ls_pc ls"      
-   
-   
+
+
 definition procedures where
-"procedures proc args \<equiv> 
+  "procedures proc args \<equiv> 
   if proc = registerUser then
     case args of 
       [String name, String mail] \<Rightarrow> 
@@ -201,19 +201,19 @@ definition procedures where
 
 
 definition latest_name_assign :: "val operationContext \<Rightarrow> val \<Rightarrow> val set" where
-"latest_name_assign ctxt u \<equiv>  {v | c1 v. 
+  "latest_name_assign ctxt u \<equiv>  {v | c1 v. 
      calls ctxt c1 \<triangleq> Call users_name_assign [u, v] Undef
    \<and> (\<forall>c2. calls ctxt c2 \<triangleq> Call users_remove [u] Undef \<longrightarrow> (c2,c1)\<in>happensBefore ctxt)
    \<and> (\<forall>c2 v'. calls ctxt c2 \<triangleq> Call users_name_assign [u] v' \<longrightarrow> \<not>(c1,c2)\<in>happensBefore ctxt)}"
 
 definition latest_mail_assign :: "val operationContext \<Rightarrow> val \<Rightarrow> val set" where
-"latest_mail_assign ctxt u \<equiv>  {v | c1 v. 
+  "latest_mail_assign ctxt u \<equiv>  {v | c1 v. 
      calls ctxt c1 \<triangleq> Call users_mail_assign [u, v] Undef
    \<and> (\<forall>c2. calls ctxt c2 \<triangleq> Call users_remove [u] Undef \<longrightarrow> (c2,c1)\<in>happensBefore ctxt)
    \<and> (\<forall>c2 v'. calls ctxt c2 \<triangleq> Call users_mail_assign [u] v' \<longrightarrow> \<not>(c1,c2)\<in>happensBefore ctxt)}"   
-   
+
 definition crdtSpec :: "operation \<Rightarrow> val list \<Rightarrow> val operationContext \<Rightarrow> val \<Rightarrow> bool" where
-"crdtSpec oper args ctxt res \<equiv> 
+  "crdtSpec oper args ctxt res \<equiv> 
   if oper \<in> {users_name_assign, users_mail_assign, users_remove} then
     (* update-operations always return Undef *)
     res = Undef
@@ -233,33 +233,33 @@ definition crdtSpec :: "operation \<Rightarrow> val list \<Rightarrow> val opera
       res \<in> latest_mail_assign ctxt (hd args)
   else
     False"
-  
+
 definition inv1 :: "val invariantContext \<Rightarrow> bool" where
-"inv1 ctxt \<equiv> \<forall>r g u.
+  "inv1 ctxt \<equiv> \<forall>r g u.
     i_invocationOp ctxt r \<triangleq> (removeUser, [u])
   \<and> i_invocationOp ctxt g \<triangleq> (getUser, [u])
   \<and> (r,g) \<in> invocation_happensBefore ctxt
   \<longrightarrow> i_invocationRes ctxt g \<triangleq> NotFound"
-  
+
 definition inv2 :: "val invariantContext \<Rightarrow> bool" where
-"inv2 ctxt \<equiv> \<forall>u i.
+  "inv2 ctxt \<equiv> \<forall>u i.
     i_invocationOp ctxt i \<triangleq> (removeUser, [u])
   \<and> i_invocationRes ctxt i \<noteq> None
   \<longrightarrow> (\<exists>c. i_callOriginI ctxt c \<triangleq> i \<and> calls ctxt c \<triangleq> Call users_remove [u] Undef)"
-  
+
 definition inv3 :: "val invariantContext \<Rightarrow> bool" where
-"inv3 ctxt \<equiv> \<not>(\<exists>write delete u v.
+  "inv3 ctxt \<equiv> \<not>(\<exists>write delete u v.
   (calls ctxt write \<triangleq> Call users_name_assign [u, v] Undef
     \<or> calls ctxt write \<triangleq> Call users_mail_assign [u, v] Undef)
   \<and> (calls ctxt delete \<triangleq> Call users_remove [u] Undef)
   \<and> (delete, write) \<in> happensBefore ctxt
   )"
-  
+
 definition inv :: "val invariantContext \<Rightarrow> bool" where
-"inv ctxt \<equiv> inv1 ctxt \<and> inv2 ctxt \<and> inv3 ctxt"
-  
+  "inv ctxt \<equiv> inv1 ctxt \<and> inv2 ctxt \<and> inv3 ctxt"
+
 definition progr :: "(localState, val) prog" where
-"progr \<equiv> \<lparr>
+  "progr \<equiv> \<lparr>
   querySpec = crdtSpec,
   procedure = procedures,
   invariant = inv
@@ -290,158 +290,257 @@ lemma procedure_cases2: "procedures procName args \<triangleq> (initState, impl)
   by (auto simp add: procedures_def split: list.splits val.splits)
 
 
+lemma StateDef_simps: 
+  "S' ::= S ==> calls S' = calls S"
+  "S' ::= S ==> happensBefore S' = happensBefore S"
+  "S' ::= S ==> prog S' = prog S"
+  "S' ::= S ==> callOrigin S' = callOrigin S"
+  "S' ::= S ==> transactionOrigin S' = transactionOrigin S"
+  "S' ::= S ==> generatedIds S' = generatedIds S"
+  "S' ::= S ==> knownIds S' = knownIds S"
+  "S' ::= S ==> invocationOp S' = invocationOp S"
+  "S' ::= S ==> invocationRes S' = invocationRes S"
+  "S' ::= S ==> transactionStatus S' = transactionStatus S"
+  "S' ::= S ==> localState S' = localState S"
+  "S' ::= S ==> currentProc S' = currentProc S"
+  "S' ::= S ==> visibleCalls S' = visibleCalls S"
+  "S' ::= S ==> currentTransaction S' = currentTransaction S"
+  by (auto simp add: Def_def)
+
+
+
+lemma IStateDef_simps: 
+  "S' ::= S ==> i_callOrigin S' = i_callOrigin S"
+  "S' ::= S ==> i_transactionOrigin S' = i_transactionOrigin S"
+  "S' ::= S ==> i_knownIds S' = i_knownIds S"
+  "S' ::= S ==> i_invocationOp S' = i_invocationOp S"
+  "S' ::= S ==> i_invocationRes S' = i_invocationRes S"
+by (auto simp add: Def_def)
+
+
 theorem "programCorrect progr"
 proof (rule show_programCorrect_using_checkCorrect)
   have [simp]: "invariant progr = inv" by (simp add: progr_def)
 
   have [simp]: "S \<in> initialStates progr i \<Longrightarrow> prog S = progr" for S i
     by (auto simp add: initialStates_def)
-  
+
+  subsection {* Initial state *}
+
+  text {* Show that the initial state satisfies the invariant *}
   show "invariant_all' (repliss_sem.initialState progr)"
-     by (auto simp add: initialState_def  inv_def inv1_def inv2_def inv3_def invContextH_def)
-  
-   show "\<And>S i. S \<in> initialStates' progr i \<Longrightarrow> invariant_all' S"
-     apply (subst(asm) initialStates'_def)
-   proof auto
+    by (auto simp add: initialState_def  inv_def inv1_def inv2_def inv3_def invContextH_def)
 
-     show "example_userbase.inv (invContextH2 (callOrigin S') (transactionOrigin S') (transactionStatus S') (happensBefore S') (calls S') (knownIds S') (invocationOp S'(i \<mapsto> (procName, args))) (invocationRes S'))" (is ?inv)
-       if i0: "prog S' = progr"
-         and i1: "procedures procName args \<triangleq> (initState, impl)"
-         and i2: "uniqueIdsInList args \<subseteq> knownIds S'"
-         and old_inv: "example_userbase.inv (invContext' S')"
-         and i4: "state_wellFormed S'"
-         and i5: "invocationOp S' i = None"
-         and i6: "\<forall>tx. transactionStatus S' tx \<noteq> Some Uncommited"
-       for  i S' procName args initState impl
-       using i1 proof (subst(asm) procedure_cases2, auto)
-       
+  subsection {* Initial state of procedure invocations *}
 
-       show "example_userbase.inv (invContextH2 (callOrigin S') (transactionOrigin S') (transactionStatus S') (happensBefore S') (calls S') (knownIds S') (invocationOp S'(i \<mapsto> (registerUser, [String name, String mail]))) (invocationRes S'))"
-         if c0: "procedures registerUser [String name, String mail] \<triangleq> (lsInit\<lparr>ls_name := name, ls_mail := mail\<rparr>, registerUserImpl)"
-           and c1: "procName = registerUser"
-           and c2: "args = [String name, String mail]"
-           and c3: "impl = registerUserImpl"
-           and c4: "initState = lsInit\<lparr>ls_name := name, ls_mail := mail\<rparr>"
-         for  name mail
-         using old_inv
-         by (auto simp add: inv_def inv1_def inv2_def inv3_def)
+  text {* Show that the initial state of procedure invocations satisfies the invariant.  *}
+  show "\<And>S i. S \<in> initialStates' progr i \<Longrightarrow> invariant_all' S"
+    apply (subst(asm) initialStates'_def)
+  proof auto
 
+    show "example_userbase.inv (invContextH2 (callOrigin S') (transactionOrigin S') (transactionStatus S') (happensBefore S') (calls S') (knownIds S') (invocationOp S'(i \<mapsto> (procName, args))) (invocationRes S'))" (is ?inv)
+      if i0: "prog S' = progr"
+        and i1: "procedures procName args \<triangleq> (initState, impl)"
+        and i2: "uniqueIdsInList args \<subseteq> knownIds S'"
+        and old_inv: "example_userbase.inv (invContext' S')"
+        and i4: "state_wellFormed S'"
+        and i5: "invocationOp S' i = None"
+        and i6: "\<forall>tx. transactionStatus S' tx \<noteq> Some Uncommited"
+      for  i S' procName args initState impl
+      using i1 proof (subst(asm) procedure_cases2, auto)
 
-       show "example_userbase.inv (invContextH2 (callOrigin S') (transactionOrigin S') (transactionStatus S') (happensBefore S') (calls S') (knownIds S') (invocationOp S'(i \<mapsto> (updateMail, [UserId u, String mail]))) (invocationRes S'))"
-         if c0: "procedures updateMail [UserId u, String mail] \<triangleq> (lsInit\<lparr>ls_u := UserId u, ls_mail := mail\<rparr>, updateMailImpl)"
-           and c1: "procName = updateMail"
-           and c2: "args = [UserId u, String mail]"
-           and c3: "impl = updateMailImpl"
-           and c4: "initState = lsInit\<lparr>ls_u := UserId u, ls_mail := mail\<rparr>"
-         for  u mail
-         using old_inv
-         by (auto simp add: inv_def inv1_def inv2_def inv3_def)
+      text {* We consider the initial state for each procedure individually: *}
 
+      paragraph {* Case registerUser *}
+      show "example_userbase.inv (invContextH2 (callOrigin S') (transactionOrigin S') (transactionStatus S') (happensBefore S') (calls S') (knownIds S') (invocationOp S'(i \<mapsto> (registerUser, [String name, String mail]))) (invocationRes S'))"
+        if c0: "procedures registerUser [String name, String mail] \<triangleq> (lsInit\<lparr>ls_name := name, ls_mail := mail\<rparr>, registerUserImpl)"
+          and c1: "procName = registerUser"
+          and c2: "args = [String name, String mail]"
+          and c3: "impl = registerUserImpl"
+          and c4: "initState = lsInit\<lparr>ls_name := name, ls_mail := mail\<rparr>"
+        for  name mail
+        using old_inv
+        by (auto simp add: inv_def inv1_def inv2_def inv3_def)
 
-       show "example_userbase.inv (invContextH2 (callOrigin S') (transactionOrigin S') (transactionStatus S') (happensBefore S') (calls S') (knownIds S') (invocationOp S'(i \<mapsto> (removeUser, [UserId u]))) (invocationRes S'))"
-         if c0: "procedures removeUser [UserId u] \<triangleq> (lsInit\<lparr>ls_u := UserId u\<rparr>, removeUserImpl)"
-           and c1: "procName = removeUser"
-           and c2: "args = [UserId u]"
-           and c3: "impl = removeUserImpl"
-           and c4: "initState = lsInit\<lparr>ls_u := UserId u\<rparr>"
-         for  u
-       proof (auto simp add: inv_def)
-         show "inv1 (invContextH2 (callOrigin S') (transactionOrigin S') (transactionStatus S') (happensBefore S') (calls S') (knownIds S') (invocationOp S'(i \<mapsto> (removeUser, [UserId u])))
+      paragraph {* Case updateMail *}
+      show "example_userbase.inv (invContextH2 (callOrigin S') (transactionOrigin S') (transactionStatus S') (happensBefore S') (calls S') (knownIds S') (invocationOp S'(i \<mapsto> (updateMail, [UserId u, String mail]))) (invocationRes S'))"
+        if c0: "procedures updateMail [UserId u, String mail] \<triangleq> (lsInit\<lparr>ls_u := UserId u, ls_mail := mail\<rparr>, updateMailImpl)"
+          and c1: "procName = updateMail"
+          and c2: "args = [UserId u, String mail]"
+          and c3: "impl = updateMailImpl"
+          and c4: "initState = lsInit\<lparr>ls_u := UserId u, ls_mail := mail\<rparr>"
+        for  u mail
+        using old_inv
+        by (auto simp add: inv_def inv1_def inv2_def inv3_def)
+
+      paragraph {* Case removeUser *}
+      show "example_userbase.inv (invContextH2 (callOrigin S') (transactionOrigin S') (transactionStatus S') (happensBefore S') (calls S') (knownIds S') (invocationOp S'(i \<mapsto> (removeUser, [UserId u]))) (invocationRes S'))"
+        if c0: "procedures removeUser [UserId u] \<triangleq> (lsInit\<lparr>ls_u := UserId u\<rparr>, removeUserImpl)"
+          and c1: "procName = removeUser"
+          and c2: "args = [UserId u]"
+          and c3: "impl = removeUserImpl"
+          and c4: "initState = lsInit\<lparr>ls_u := UserId u\<rparr>"
+        for  u
+      proof (auto simp add: inv_def)
+        show "inv1 (invContextH2 (callOrigin S') (transactionOrigin S') (transactionStatus S') (happensBefore S') (calls S') (knownIds S') (invocationOp S'(i \<mapsto> (removeUser, [UserId u])))
            (invocationRes S'))"
-           using old_inv
-           apply (auto simp add: inv_def inv1_def)[1]
-           using i4 i5 new_invocation_cannot_happen_before by blast
+          using old_inv
+          apply (auto simp add: inv_def inv1_def)[1]
+          using i4 i5 new_invocation_cannot_happen_before by blast
 
 
-          show "inv2 (invContextH2 (callOrigin S') (transactionOrigin S') (transactionStatus S') (happensBefore S') (calls S') (knownIds S') (invocationOp S'(i \<mapsto> (removeUser, [UserId u])))
+        show "inv2 (invContextH2 (callOrigin S') (transactionOrigin S') (transactionStatus S') (happensBefore S') (calls S') (knownIds S') (invocationOp S'(i \<mapsto> (removeUser, [UserId u])))
            (invocationRes S'))"
 
-            using old_inv
-            apply (auto simp add: inv_def inv2_def)
-            by (simp add: i4 i5 state_wellFormed_invocation_before_result)
+          using old_inv
+          apply (auto simp add: inv_def inv2_def)
+          by (simp add: i4 i5 state_wellFormed_invocation_before_result)
 
-          show "inv3 (invContextH2 (callOrigin S') (transactionOrigin S') (transactionStatus S') (happensBefore S') (calls S') (knownIds S') (invocationOp S'(i \<mapsto> (removeUser, [UserId u])))
+        show "inv3 (invContextH2 (callOrigin S') (transactionOrigin S') (transactionStatus S') (happensBefore S') (calls S') (knownIds S') (invocationOp S'(i \<mapsto> (removeUser, [UserId u])))
            (invocationRes S'))"
-            using old_inv
-            by (auto simp add: inv_def inv3_def)
-        qed
+          using old_inv
+          by (auto simp add: inv_def inv3_def)
+      qed
 
 
+      paragraph {* Case getUser *}
+      show "example_userbase.inv (invContextH2 (callOrigin S') (transactionOrigin S') (transactionStatus S') (happensBefore S') (calls S') (knownIds S') (invocationOp S'(i \<mapsto> (getUser, [UserId u]))) (invocationRes S'))"
+        if c0: "procedures getUser [UserId u] \<triangleq> (lsInit\<lparr>ls_u := UserId u\<rparr>, getUserImpl)"
+          and c1: "procName = getUser"
+          and c2: "args = [UserId u]"
+          and c3: "impl = getUserImpl"
+          and c4: "initState = lsInit\<lparr>ls_u := UserId u\<rparr>"
+        for  u
+      proof (auto simp add: inv_def)
 
-
-        show "example_userbase.inv (invContextH2 (callOrigin S') (transactionOrigin S') (transactionStatus S') (happensBefore S') (calls S') (knownIds S') (invocationOp S'(i \<mapsto> (getUser, [UserId u]))) (invocationRes S'))"
-          if c0: "procedures getUser [UserId u] \<triangleq> (lsInit\<lparr>ls_u := UserId u\<rparr>, getUserImpl)"
-            and c1: "procName = getUser"
-            and c2: "args = [UserId u]"
-            and c3: "impl = getUserImpl"
-            and c4: "initState = lsInit\<lparr>ls_u := UserId u\<rparr>"
-          for  u
-        proof (auto simp add: inv_def)
-
-          from old_inv
-          show "inv1 (invContextH2 (callOrigin S') (transactionOrigin S') (transactionStatus S') (happensBefore S') (calls S') (knownIds S') (invocationOp S'(i \<mapsto> (getUser, [UserId u])))
+        from old_inv
+        show "inv1 (invContextH2 (callOrigin S') (transactionOrigin S') (transactionStatus S') (happensBefore S') (calls S') (knownIds S') (invocationOp S'(i \<mapsto> (getUser, [UserId u])))
              (invocationRes S'))"
-            apply (auto simp add: inv_def inv1_def)
-            using i4 i5 new_invocation_cannot_happen_after by blast
+          apply (auto simp add: inv_def inv1_def)
+          using i4 i5 new_invocation_cannot_happen_after by blast
 
-          from old_inv
-          show "inv2 (invContextH2 (callOrigin S') (transactionOrigin S') (transactionStatus S') (happensBefore S') (calls S') (knownIds S') (invocationOp S'(i \<mapsto> (getUser, [UserId u])))
+        from old_inv
+        show "inv2 (invContextH2 (callOrigin S') (transactionOrigin S') (transactionStatus S') (happensBefore S') (calls S') (knownIds S') (invocationOp S'(i \<mapsto> (getUser, [UserId u])))
              (invocationRes S'))"
-            by (auto simp add: inv_def inv2_def)
+          by (auto simp add: inv_def inv2_def)
 
-          from old_inv
-          show "inv3 (invContextH2 (callOrigin S') (transactionOrigin S') (transactionStatus S') (happensBefore S') (calls S') (knownIds S') (invocationOp S'(i \<mapsto> (getUser, [UserId u])))
+        from old_inv
+        show "inv3 (invContextH2 (callOrigin S') (transactionOrigin S') (transactionStatus S') (happensBefore S') (calls S') (knownIds S') (invocationOp S'(i \<mapsto> (getUser, [UserId u])))
              (invocationRes S'))"
-            by (auto simp add: inv_def inv3_def)
-        qed
+          by (auto simp add: inv_def inv3_def)
       qed
     qed
+  qed
+
+  subsection {* We check the implementation using the checkCorrect2F function. 
+       This basically checks the implementation up to the given bound.
+       We have to show that there exists a bound such that all reachable states are covered and proven correct.  *}
+  show "\<exists>bound. (checkCorrect2F ^^ bound) bot (progr, {}, S, i)"
+    if c0: "S \<in> initialStates' progr i"
+    for  S i
+
+    text {* We unfold the definition of initial states. *}
+    using c0  apply (subst(asm) initialStates'_def)
+  proof auto
 
 
-    show "\<exists>bound. (checkCorrect2F ^^ bound) bot (progr, {}, S, i)"
-      if c0: "S \<in> initialStates' progr i"
-      for  S i
+    show "\<exists>bound. (checkCorrect2F ^^ bound) bot (progr, {}, Sa \<lparr>localState := localState Sa(i \<mapsto> initState), currentProc := currentProc Sa(i \<mapsto> impl), visibleCalls := visibleCalls Sa(i \<mapsto> {}), invocationOp := invocationOp Sa(i \<mapsto> (procName, args))\<rparr>, i)"
+      if c0: "S = Sa\<lparr>localState := localState Sa(i \<mapsto> initState), currentProc := currentProc Sa(i \<mapsto> impl), visibleCalls := visibleCalls Sa(i \<mapsto> {}), invocationOp := invocationOp Sa(i \<mapsto> (procName, args))\<rparr>"
+        and c1: "prog Sa = progr"
+        and c2: "procedures procName args \<triangleq> (initState, impl)"
+        and c3: "uniqueIdsInList args \<subseteq> knownIds Sa"
+        and c4: "example_userbase.inv (invContext' Sa)"
+        and c5: "state_wellFormed Sa"
+        and c6: "invocationOp Sa i = None"
+        and c7: "\<forall>tx. transactionStatus Sa tx \<noteq> Some Uncommited"
+      for  Sa procName args initState impl
+      text {* We consider the case for each procedure separately:  *}
+      using c2 proof (subst(asm) procedure_cases2, auto)
 
-      using c0  apply (subst(asm) initialStates'_def)
-    proof auto
+      have [simp]: "currentTransaction Sa i = None"
+        by (simp add: c5 c6 wellFormed_invoc_notStarted(1))
+
+(* ony unfold definitions, when needed for evaluation: *)
+      have h1[simp]:  "S' ::= S \<Longrightarrow> (currentProc S' i \<triangleq> x) \<longleftrightarrow> (currentProc S i \<triangleq> x)" for S' S i x  by (auto simp add: Def_def)
+      have h2[simp]: "S' ::= S \<Longrightarrow>  ls_pc (the (localState S' i)) = ls_pc (the (localState S i))" for S' S i by (auto simp add: Def_def)
+      have h3[simp]: "S' ::= S \<Longrightarrow>  (currentTransaction S' i = None) \<longleftrightarrow> (currentTransaction S i = None)" for S' S i by (auto simp add: Def_def)
+
+      have queries_defined_users_name_assign[simp]: 
+        "Ex (querySpec progr users_name_assign [u, n] ctxt)"
+        for u n ctxt
+        by (auto simp add: progr_def crdtSpec_def )
+
+      have queries_defined_users_name_assign[simp]: 
+        "Ex (querySpec progr users_mail_assign [u, n] ctxt)"
+        for u n ctxt
+        by (auto simp add: progr_def crdtSpec_def )
+
+      paragraph {* Case register User: *}
+      show "\<exists>bound. (checkCorrect2F ^^ bound) bot (progr, {}, Sa \<lparr>localState := localState Sa(i \<mapsto> lsInit\<lparr>ls_name := name, ls_mail := mail\<rparr>), currentProc := currentProc Sa(i \<mapsto> registerUserImpl), visibleCalls := visibleCalls Sa(i \<mapsto> {}), invocationOp := invocationOp Sa(i \<mapsto> (registerUser, [String name, String mail]))\<rparr>, i)"
+        if c0: "procedures registerUser [String name, String mail] \<triangleq> (lsInit\<lparr>ls_name := name, ls_mail := mail\<rparr>, registerUserImpl)"
+          and c1: "procName = registerUser"
+          and c2: "args = [String name, String mail]"
+          and c3: "impl = registerUserImpl"
+          and c4: "initState = lsInit\<lparr>ls_name := name, ls_mail := mail\<rparr>"
+        for  name mail
+        text {* We start by unrolling the implementation. *}
+        apply (rule_tac x="10" in exI)
+        apply (rule checkCorrect2F_step, auto simp add: registerUserImpl_def lsInit_def split: localAction.splits option.splits)
+        apply (rule checkCorrect2F_step, auto simp add: registerUserImpl_def lsInit_def split: localAction.splits option.splits)
+        apply (rule checkCorrect2F_step, auto simp add: registerUserImpl_def lsInit_def split: localAction.splits option.splits)
+        apply (rule checkCorrect2F_step, auto simp add: registerUserImpl_def lsInit_def split: localAction.splits option.splits)
+        apply (rule checkCorrect2F_step, auto simp add: registerUserImpl_def lsInit_def split: localAction.splits option.splits)
+         defer
+         apply (rule checkCorrect2F_step, auto simp add: registerUserImpl_def lsInit_def split: localAction.splits option.splits)
+      proof -
+        fix uid S' t S'a newTxns S'' vis' ls x2 c res S'b vis'a hb' x2a ca resa S'c vis'b hb'a x2b S'd S'e
+        assume a0: "uid \<notin> generatedIds Sa"
+          and a1: "S' ::= Sa         \<lparr>currentProc := currentProc Sa(i \<mapsto> registerUserImpl), visibleCalls := visibleCalls Sa(i \<mapsto> {}),            invocationOp := invocationOp Sa(i \<mapsto> (registerUser, [String name, String mail])),            localState := localState Sa(i \<mapsto> \<lparr>ls_pc = Suc 0, ls_u = uid, ls_name = name, ls_mail = mail, ls_exists = False\<rparr>),            generatedIds := insert uid (generatedIds Sa)\<rparr>"
+          and a2: "localState S' i \<triangleq> ls"
+          and a3: "transactionStatus S' t = None"
+          and a4: "prog S'a = prog S'"
+          and a5: "invariant (prog S') (invContext' S'a)"
+          and a6: "\<forall>tx. transactionStatus S'a tx \<noteq> Some Uncommited"
+          and a7: "state_wellFormed S'a"
+          and a8: "state_wellFormed S''"
+          and a9: "state_monotonicGrowth S' S'a"
+          and a10: "localState S'a i \<triangleq> ls"
+          and a11: "currentProc S'a i \<triangleq> registerUserImpl"
+          and a12: "currentTransaction S'a i = None"
+          and a13: "visibleCalls S' i \<triangleq> {}"
+          and a14: "visibleCalls S'a i \<triangleq> {}"
+          and a15: "vis' ::= callsInTransaction S'a newTxns \<down> happensBefore S'a"
+          and a16: "newTxns \<subseteq> dom (transactionStatus S'a)"
+          and a17: "consistentSnapshot S'a vis'"
+          and a18: "transactionStatus S'a t = None"
+          and a19: "\<forall>c. callOrigin S'a c \<noteq> Some t"
+          and a20: "transactionOrigin S'a t = None"
+          and a21: "S'' ::= S'a         \<lparr>transactionStatus := transactionStatus S'a(t \<mapsto> Uncommited), transactionOrigin := transactionOrigin S'a(t \<mapsto> i),            currentTransaction := currentTransaction S'a(i \<mapsto> t), localState := localState S'a(i \<mapsto> ls\<lparr>ls_pc := 2\<rparr>), visibleCalls := visibleCalls S'a(i \<mapsto> vis')\<rparr>"
+          and a22: "currentTransaction S'' i \<triangleq> x2"
+          and a23: "calls S'' c = None"
+          and a24: "querySpec progr users_name_assign [ls_u (the (localState S'' i)), String (ls_name (the (localState S'' i)))]          (getContextH (calls S'') (happensBefore S'') (Some vis')) res"
+          and a25: "visibleCalls S'' i \<triangleq> vis'"
+          and a26: "vis'a ::= visibleCalls S''(i \<mapsto> insert c vis')"
+          and a27: "hb' ::= updateHb (happensBefore S'') vis' [c]"
+          and a28: "S'b ::= S''         \<lparr>localState := localState S''(i \<mapsto> the (localState S'' i)\<lparr>ls_pc := 3\<rparr>),            calls := calls S''(c \<mapsto> Call users_name_assign [ls_u (the (localState S'' i)), String (ls_name (the (localState S'' i)))] res),            callOrigin := callOrigin S''(c \<mapsto> x2), visibleCalls := vis'a, happensBefore := hb'\<rparr>"
+          and a29: "currentTransaction S'b i \<triangleq> x2a"
+          and a30: "calls S'b ca = None"
+          and a31: "querySpec progr users_mail_assign [ls_u (the (localState S'b i)), String (ls_mail (the (localState S'b i)))]          (getContextH (calls S'b) (happensBefore S'b) (Some (insert c vis'))) resa"
+          and a32: "visibleCalls S'b i \<triangleq> insert c vis'"
+          and a33: "vis'b ::= visibleCalls S'b(i \<mapsto> insert ca (insert c vis'))"
+          and a34: "hb'a ::= updateHb (happensBefore S'b) (insert c vis') [ca]"
+          and a35: "S'c ::= S'b         \<lparr>localState := localState S'b(i \<mapsto> the (localState S'b i)\<lparr>ls_pc := 4\<rparr>),            calls := calls S'b(ca \<mapsto> Call users_mail_assign [ls_u (the (localState S'b i)), String (ls_mail (the (localState S'b i)))] resa),            callOrigin := callOrigin S'b(ca \<mapsto> x2a), visibleCalls := vis'b, happensBefore := hb'a\<rparr>"
+          and a36: "currentTransaction S'c i \<triangleq> x2b"
+          and a37: "S'd ::= S'c         \<lparr>localState := localState S'c(i \<mapsto> the (localState S'c i)\<lparr>ls_pc := 5\<rparr>), currentTransaction := (currentTransaction S'c)(i := None),            transactionStatus := transactionStatus S'c(x2b \<mapsto> Commited)\<rparr>"
+          and a38: "\<forall>t. transactionStatus S'd t \<noteq> Some Uncommited"
+          and a39: "example_userbase.inv (invContext' S'd)"
+          and a40: "S'e ::= S'd         \<lparr>localState := (localState S'd)(i := None), currentProc := (currentProc S'd)(i := None), visibleCalls := (visibleCalls S'd)(i := None),            invocationRes := invocationRes S'd(i \<mapsto> ls_u (the (localState S'd i))), knownIds := knownIds S'd \<union> uniqueIds (ls_u (the (localState S'd i)))\<rparr>"
+          and a41: "\<forall>t. transactionStatus S'e t \<noteq> Some Uncommited"
+
+        show "example_userbase.inv (invContext' S'e)"
+          sorry
 
 
-      show "\<exists>bound. (checkCorrect2F ^^ bound) bot (progr, {}, Sa \<lparr>localState := localState Sa(i \<mapsto> initState), currentProc := currentProc Sa(i \<mapsto> impl), visibleCalls := visibleCalls Sa(i \<mapsto> {}), invocationOp := invocationOp Sa(i \<mapsto> (procName, args))\<rparr>, i)"
-        if c0: "S = Sa\<lparr>localState := localState Sa(i \<mapsto> initState), currentProc := currentProc Sa(i \<mapsto> impl), visibleCalls := visibleCalls Sa(i \<mapsto> {}), invocationOp := invocationOp Sa(i \<mapsto> (procName, args))\<rparr>"
-          and c1: "prog Sa = progr"
-          and c2: "procedures procName args \<triangleq> (initState, impl)"
-          and c3: "uniqueIdsInList args \<subseteq> knownIds Sa"
-          and c4: "example_userbase.inv (invContext' Sa)"
-          and c5: "state_wellFormed Sa"
-          and c6: "invocationOp Sa i = None"
-          and c7: "\<forall>tx. transactionStatus Sa tx \<noteq> Some Uncommited"
-        for  Sa procName args initState impl
-        using c2 proof (subst(asm) procedure_cases2, auto)
-
-        have [simp]: "currentTransaction Sa i = None"
-          by (simp add: c5 c6 wellFormed_invoc_notStarted(1))
-
-
-
-        show "\<exists>bound. (checkCorrect2F ^^ bound) bot (progr, {}, Sa \<lparr>localState := localState Sa(i \<mapsto> lsInit\<lparr>ls_name := name, ls_mail := mail\<rparr>), currentProc := currentProc Sa(i \<mapsto> registerUserImpl), visibleCalls := visibleCalls Sa(i \<mapsto> {}), invocationOp := invocationOp Sa(i \<mapsto> (registerUser, [String name, String mail]))\<rparr>, i)"
-          if c0: "procedures registerUser [String name, String mail] \<triangleq> (lsInit\<lparr>ls_name := name, ls_mail := mail\<rparr>, registerUserImpl)"
-            and c1: "procName = registerUser"
-            and c2: "args = [String name, String mail]"
-            and c3: "impl = registerUserImpl"
-            and c4: "initState = lsInit\<lparr>ls_name := name, ls_mail := mail\<rparr>"
-          for  name mail
-          apply (rule_tac x="10" in exI)
-          apply (rule checkCorrect2F_step, auto simp add: registerUserImpl_def lsInit_def split: localAction.splits option.splits)
-          apply (rule checkCorrect2F_step, auto simp add: registerUserImpl_def lsInit_def split: localAction.splits option.splits)
-          apply (rule checkCorrect2F_step, auto simp add: registerUserImpl_def lsInit_def split: localAction.splits option.splits)
-          apply (auto simp add: progr_def crdtSpec_def )[1]
-          apply (rule checkCorrect2F_step, auto simp add: registerUserImpl_def lsInit_def split: localAction.splits option.splits)
-           apply (auto simp add: progr_def crdtSpec_def )[1]
-          apply (rule checkCorrect2F_step, auto simp add: registerUserImpl_def lsInit_def split: localAction.splits option.splits)
-           defer
-           apply (rule checkCorrect2F_step, auto simp add: registerUserImpl_def lsInit_def split: localAction.splits option.splits)
-
-        proof
 
 
 
@@ -451,89 +550,78 @@ proof (rule show_programCorrect_using_checkCorrect)
 
 
 
+        show "programCorrect_s progr"
+        proof (rule show_program_correct_single_invocation)
+          show "\<And>S i. S \<in> initialStates progr i \<Longrightarrow> invariant_all S"
+          proof (auto simp add: invariant_all_def inv_def)
+            fix S i vis
+            assume a0: "S \<in> initialStates progr i"
+              and vis_cs: "consistentSnapshot S vis"
+
+
+            from a0 
+            obtain Spre procName args initState impl
+              where S_def: "S = Spre\<lparr>localState := localState Spre(i \<mapsto> initState), currentProc := currentProc Spre(i \<mapsto> impl), visibleCalls := visibleCalls Spre(i \<mapsto> {}), invocationOp := invocationOp Spre(i \<mapsto> (procName, args))\<rparr>"
+                and a1: "prog Spre = progr"
+                and a2: "procedure progr procName args \<triangleq> (initState, impl)"
+                and a3: "uniqueIdsInList args \<subseteq> knownIds Spre"
+                and pre_inv_all: "invariant_all Spre"
+                and pre_wf: "state_wellFormed Spre"
+                and a6: "invocationOp Spre i = None"
+              by (subst(asm) initialStates_def, auto)
+
+            from `consistentSnapshot S vis` 
+            have vis_cs_pre: "consistentSnapshot Spre vis"
+              by (auto simp add: consistentSnapshot_def S_def)
+
+            from pre_inv_all
+            have pre_inv: "inv (invContextVis Spre vis)"
+              by (auto simp add: invariant_all_def `prog Spre = progr` `consistentSnapshot Spre vis`)
+
+
+            from pre_inv 
+            have "inv1 (invContextVis Spre vis)"
+              using example_userbase.inv_def by blast
+            thus "inv1 (invContextVis S vis)"
+              apply (auto simp add: inv1_def  split: if_splits)
+              apply (auto simp add: invariant_simps)
+
+
+              apply (auto simp add: invContextH_def invocation_happensBefore_def i_callOriginI_def )
+
+
+
+              apply (subst(asm) invariantContext.simps)+
+              apply (auto simp add: restrict_relation_def restrict_map_def)
+
+              find_theorems i_transactionOrigin
+              apply (drule_tac x=r in spec)
+              apply (drule_tac x=g in spec)
+              sorry (* apply (auto simp add: invocation_happensBefore_def) *)
+
+(* TODO add simplification rules for "i_invocationOp (invContextVis S vis)" and other fields *)
+
+
+            show "inv2 (invContextVis S vis)"
+              using a0 apply (subst(asm) initialStates_def)
+              apply (auto simp add: inv2_def invContextH_def restrict_relation_def restrict_map_def i_callOriginI_def invariantContext.defs split: if_splits option.splits)
+              apply (simp add: state_wellFormed_invocation_before_result)
+              sorry
+
+            show "inv3 (invContextVis S vis)"
+              using a0 apply (subst(asm) initialStates_def)
+              apply (auto simp add: inv3_def  invContextH_def restrict_relation_def restrict_map_def  split: if_splits)
+
+
+              sorry
+
+            show "\<And>bound S i. S \<in> initialStates progr i \<Longrightarrow> checkCorrect progr S i bound"
 
 
 
 
-
-
-
-
-
-
-     
-  show "programCorrect_s progr"
-  proof (rule show_program_correct_single_invocation)
-    show "\<And>S i. S \<in> initialStates progr i \<Longrightarrow> invariant_all S"
-    proof (auto simp add: invariant_all_def inv_def)
-      fix S i vis
-      assume a0: "S \<in> initialStates progr i"
-         and vis_cs: "consistentSnapshot S vis"
-      
-      
-      from a0 
-      obtain Spre procName args initState impl
-        where S_def: "S = Spre\<lparr>localState := localState Spre(i \<mapsto> initState), currentProc := currentProc Spre(i \<mapsto> impl), visibleCalls := visibleCalls Spre(i \<mapsto> {}), invocationOp := invocationOp Spre(i \<mapsto> (procName, args))\<rparr>"
-          and a1: "prog Spre = progr"
-          and a2: "procedure progr procName args \<triangleq> (initState, impl)"
-          and a3: "uniqueIdsInList args \<subseteq> knownIds Spre"
-          and pre_inv_all: "invariant_all Spre"
-          and pre_wf: "state_wellFormed Spre"
-          and a6: "invocationOp Spre i = None"
-      by (subst(asm) initialStates_def, auto)
-
-      from `consistentSnapshot S vis` 
-      have vis_cs_pre: "consistentSnapshot Spre vis"
-        by (auto simp add: consistentSnapshot_def S_def)
-      
-      from pre_inv_all
-      have pre_inv: "inv (invContextVis Spre vis)"
-        by (auto simp add: invariant_all_def `prog Spre = progr` `consistentSnapshot Spre vis`)
-        
-      
-      from pre_inv 
-      have "inv1 (invContextVis Spre vis)"
-        using example_userbase.inv_def by blast
-      thus "inv1 (invContextVis S vis)"
-        apply (auto simp add: inv1_def  split: if_splits)
-        apply (auto simp add: invariant_simps)
-        
-        
-        apply (auto simp add: invContextH_def invocation_happensBefore_def i_callOriginI_def )
-        
-        
-        
-        apply (subst(asm) invariantContext.simps)+
-        apply (auto simp add: restrict_relation_def restrict_map_def)
-        
-        find_theorems i_transactionOrigin
-        apply (drule_tac x=r in spec)
-        apply (drule_tac x=g in spec)
-        sorry (* apply (auto simp add: invocation_happensBefore_def) *)
-       
-        (* TODO add simplification rules for "i_invocationOp (invContextVis S vis)" and other fields *)
-        
-      
-      show "inv2 (invContextVis S vis)"
-        using a0 apply (subst(asm) initialStates_def)
-        apply (auto simp add: inv2_def invContextH_def restrict_relation_def restrict_map_def i_callOriginI_def invariantContext.defs split: if_splits option.splits)
-        apply (simp add: state_wellFormed_invocation_before_result)
-        sorry
-        
-      show "inv3 (invContextVis S vis)"
-        using a0 apply (subst(asm) initialStates_def)
-        apply (auto simp add: inv3_def  invContextH_def restrict_relation_def restrict_map_def  split: if_splits)
-        
-        
-      sorry
-    
-    show "\<And>bound S i. S \<in> initialStates progr i \<Longrightarrow> checkCorrect progr S i bound"
-    
-      
-    
-  
-  apply (auto simp add: programCorrect_s_def)
-  apply (auto simp add: prog_def step_s.simps)
+              apply (auto simp add: programCorrect_s_def)
+              apply (auto simp add: prog_def step_s.simps)
 
 
 
